utp/utp_expr.thy
@@ -129,6 +129,12 @@ begin
   definition plus_uexpr_def: "u + v = bop (op +) u v"
 instance ..
 end
+  
+instantiation uexpr :: (dzero, type) dzero
+begin
+  definition dzero_uexpr_def: "dzero u = uop dzero u"
+instance ..
+end
 
 text \<open> It should be noted that instantiating the unary minus class, @{class uminus}, will also 
   provide negation UTP predicates later. \<close>
@@ -590,6 +596,7 @@ lemmas uexpr_defs =
   ulim_right_def
   ucont_on_def
   plus_list_def
+  dzero_uexpr_def
   
 text \<open> The following laws show how to evaluate the core expressions constructs in terms of which
   the above definitions are defined. Thus, using these theorems together, we can convert any UTP 
