utils/utp_imports.thy
@@ -27,7 +27,6 @@ imports
   "Library_extra/Monoid_extra"
   "Library_extra/Pfun"
   "Library_extra/Ffun"
-  "Library_extra/Terminated_lists"
   Profiling
   TotalRecall
 begin end
